Mica/TinyML/Printer.lean
@@ -15,6 +15,7 @@ def Typ.print : Typ → String
   | .arrow t1 t2 => s!"{wrapArg t1 (Typ.print t1)} -> {Typ.print t2}"
   | .ref t => s!"ref {wrapArg t (Typ.print t)}"
   | .array t => s!"array {wrapArg t (Typ.print t)}"
+  | .ownedArray t => s!"owned-array {wrapArg t (Typ.print t)}"
   | .vec t => s!"vec {wrapArg t (Typ.print t)}"
   | .owned t => s!"owned {wrapArg t (Typ.print t)}"
   | .empty => "empty"
